theories/singletons.v
@@ -83,10 +83,10 @@ refine (fun q α => _). unshelve econstructor.
   exact (wedge_eq ((α ∘ β) · A0) ((α ∘ β) · A1) ((α ∘ β) · a0) ((α ∘ β) · a1) ((α ∘ β) · b0) ((α ∘ β) · b1) ((α ∘ β) · e0) ((α ∘ β) · e1)).
 - unshelve refine (fun r β s => _). simpl in s.
   exact (wedge_eqR ((α ∘ β) · A0) ((α ∘ β) · A1) ((α ∘ β) · a0) ((α ∘ β) · a1) ((α ∘ β) · b0) ((α ∘ β) · b1) ((α ∘ β) · e0) ((α ∘ β) · e1) s).
-- refine (fun r β s0 s1 => _). apply falso.
-- refine (fun r β s0 s1 => _). apply falso.
-- refine (fun r β s0 s1 => _). apply sfalso.
-- refine (fun r β s0 s1 => _). apply sfalso.
+- refine (fun r β c s0 s1 => _). apply falso.
+- refine (fun r β c s0 s1 => _). apply falso.
+- refine (fun r β c s0 s1 => _). apply sfalso.
+- refine (fun r β c s0 s1 => _). apply sfalso.
 Defined.
 
 Definition contractor1 {p}
@@ -100,7 +100,7 @@ Definition contractor1 {p}
   (e1 : El1 _ (eq1 A0 A1 a0 a1 b0 b1) e0)
   : @El1 p Type0 Type1 (contractor0 A0 A1 a0 a1 b0 b1 e0 e1).
 Proof.
-refine (fun q α => _).
+refine (fun q α r β => _).
 reflexivity.
 Defined.
 
